proof/schnorr_protocol/side_channel_properties/Challenge_LF.ec
@@ -5,278 +5,15 @@ from Jasmin require import JModel.
 require import AuxLemmas.
 require import Ops_LeakageFunctions.
 
-(* SAMPLING LEAKAGES  *)
+
 require import W64_SchnorrExtract_ct.
 module M1 = W64_SchnorrExtract_ct.M(W64_SchnorrExtract_ct.Syscall).
 
-require Constants.
-op challenge_t i : leakages_t =  samp_t i ++ ([LeakAddr []] ++ bn_set_q_t ++ [LeakAddr []]).
 
-lemma challenge_t_inj : injective challenge_t.
-move => x y.
-have : x <> y => challenge_t x <> challenge_t y.
-move => xneqy.
-rewrite /commitment_t.
-have : samp_t x <> samp_t y. smt(samp_t_inj).
-smt(@List).
-smt().
-qed.
-
-
-lemma challenge_leakages2   &m : (glob M1){m} = [] =>
-  Pr[ M1.challenge_indexed() @ &m : M1.leakages <> challenge_t res.`1 ] = 0%r.
-progress. byphoare (_: glob M1 = [] ==> _).
+lemma challenge_leakages_ph start_l : 
+  phoare [ M(Syscall).challenge : M.leakages = start_l ==> M.leakages <> challenge_t ++ start_l] = 0%r.
 hoare. simplify.
-proc.
-pose suf1 :=  [LeakAddr []].
-seq 5 : (M.leakages = bn_set_q_t ++ suf1 ).
-wp.  call (bn_set_q_leakages suf1). simplify. wp. skip. progress. 
-pose suf2 := [LeakAddr []] ++ bn_set_q_t ++ suf1.
-seq 4 : (M.leakages = samp_t i ++ suf2).
-wp. call  (rsample_leakages suf2). wp.
-skip. progress. skip. progress.
-rewrite /challenge_t /suf2 /suf1.
-auto. auto.
-qed.
-
-
-lemma challenge_leakages3 l x &m : (glob M1){m} = [] =>
-  Pr[ M1.challenge_indexed() @ &m : M1.leakages = l  /\ res.`2 = x ]
-  = Pr[ M1.challenge_indexed() @ &m : l = challenge_t res.`1 /\ res.`2 = x  ].
-move => H.
-have ->: Pr[ M1.challenge_indexed() @ &m : l = challenge_t res.`1 /\ res.`2 = x ]
- = Pr[ M1.challenge_indexed() @ &m : l = challenge_t res.`1 /\ res.`2 = x /\ M1.leakages = challenge_t res.`1  ].
-  have -> : Pr[M1.challenge_indexed() @ &m : l = challenge_t res.`1 /\ res.`2 = x]
-   = Pr[M1.challenge_indexed() @ &m : l = challenge_t res.`1 /\ res.`2 = x /\ M1.leakages = challenge_t res.`1]
-   + Pr[M1.challenge_indexed() @ &m : l = challenge_t res.`1 /\ res.`2 = x /\ M1.leakages <> challenge_t res.`1].
-   rewrite Pr[mu_split (M1.leakages = challenge_t res.`1)]. smt(). 
-  have ->: Pr[M1.challenge_indexed() @ &m :
-   l = challenge_t res.`1 /\ res.`2 = x /\ M1.leakages <> challenge_t res.`1] = 0%r.
-    have : Pr[M1.challenge_indexed() @ &m :
-       l = challenge_t res.`1 /\ res.`2 = x /\ M1.leakages <> challenge_t res.`1]
-     <= Pr[ M1.challenge_indexed() @ &m : M1.leakages <> challenge_t res.`1 ]. smt(@Distr).
-    rewrite (challenge_leakages2  &m). auto. smt(@Distr). 
-auto.
-have -> : Pr[ M1.challenge_indexed() @ &m : l = challenge_t res.`1 /\ res.`2 = x /\ M1.leakages = challenge_t res.`1  ]
- = Pr[ M1.challenge_indexed() @ &m : res.`2 = x /\  l = M1.leakages /\ M1.leakages = challenge_t res.`1  ].
-rewrite Pr[mu_eq]. move => &hr. split.  smt().  smt(). auto.
-have -> : Pr[ M1.challenge_indexed() @ &m : res.`2 = x /\ l = M1.leakages /\ M1.leakages = challenge_t res.`1  ]
- = Pr[ M1.challenge_indexed() @ &m :  l = M1.leakages /\ res.`2 = x ].
-  have : Pr[ M1.challenge_indexed() @ &m :  l = M1.leakages /\ res.`2 = x ] 
-   = Pr[ M1.challenge_indexed() @ &m :  l = M1.leakages /\ res.`2 = x /\ M1.leakages = challenge_t res.`1  ]
-   + Pr[ M1.challenge_indexed() @ &m :  l = M1.leakages /\ res.`2 = x /\ M1.leakages <> challenge_t res.`1  ].
- rewrite Pr[mu_split (M1.leakages = challenge_t res.`1 )]. smt().
-   have : Pr[ M1.challenge_indexed() @ &m :  l = M1.leakages /\ res.`2 = x /\ M1.leakages <> challenge_t res.`1  ]
-    = 0%r.
-     have : Pr[ M1.challenge_indexed() @ &m :  l = M1.leakages /\ res.`2 = x /\ M1.leakages <> challenge_t res.`1  ] 
-         <= Pr[ M1.challenge_indexed() @ &m : M1.leakages <> challenge_t res.`1 ].
-       rewrite Pr[mu_sub]. auto. auto.
-    rewrite (challenge_leakages2 &m). auto. smt(@Distr).
-    move => h. rewrite h. simplify. progress. rewrite H0.
-rewrite Pr[mu_eq]. smt(). auto. 
-rewrite Pr[mu_eq]. smt(). auto.
-qed.
-
-
-lemma challenge_leakages_inv x l &m : (glob M1){m} = [] 
- => Pr[ M1.challenge_indexed() @ &m : M1.leakages = l /\ res.`2 = x  ]
-  = Pr[ M1.challenge_indexed() @ &m :  (inv (-1) challenge_t) l = res.`1  /\ res.`2 = x  ].
-move => ic (* ic' *). rewrite  (challenge_leakages3 l x &m). auto. auto.
-simplify. 
-have -> : 
-  Pr[M1.challenge_indexed() @ &m :
-   l = challenge_t res.`1 /\ res.`2 = x]
-  =   Pr[M1.challenge_indexed() @ &m :
-   l = challenge_t res.`1 /\ res.`2 = x /\ 0 <= res.`1]. 
-byequiv.
-proc. inline M(Syscall).bn_rsample. wp.
-while (0 <= i0{1} /\ ={i0,byte_p, byte_z}). wp.  simplify.
-call (_: true).  wp. sim. wp. 
-call (_:true). sim. wp. 
-call (_:true).  sim. wp. 
-skip. progress. smt(). wp.
-call (_: true).  sim. wp.
-call (_: true ).  sim. wp.
-skip. progress. auto. auto.
-have -> : Pr[M1.challenge_indexed() @ &m :
-   inv (-1) challenge_t l = res.`1 /\ res.`2 = x] 
- = Pr[M1.challenge_indexed() @ &m :
-   inv (-1) challenge_t l = res.`1 /\ res.`2 = x /\ 0 <= res.`1].
-byequiv.
-proc. inline M(Syscall).bn_rsample. wp.
-while (0 <= i0{1} /\ ={i0,byte_p, byte_z}). wp.  simplify.
-call (_: true).  wp. sim. wp. 
-call (_:true). sim. wp. 
-call (_:true).  sim. wp. 
-skip. progress. smt(). wp.
-call (_: true).  sim. wp.
-call (_: true ).  sim. wp.
-skip. progress. auto. auto.
-rewrite Pr[mu_eq].
-progress.
-rewrite invP. apply challenge_t_inj. auto.  
-have : exists z, (challenge_t z) = l.
-apply (choiceEx (-1) challenge_t l res{hr}.`1) . apply H. smt().
-elim. progress.
-rewrite - H.
-rewrite invP.
-apply challenge_t_inj. auto.
-auto.
-qed.
-
-
-require import W64_SchnorrExtract.
-module M2 = W64_SchnorrExtract.M(W64_SchnorrExtract.Syscall).  
-
-lemma M1_M2_challenge :
-  equiv  [ M1.challenge_indexed ~ M2.challenge_indexed
-    : true ==> ={res}  ].
-proof. proc.
-seq 6 3  : (={exp_order}).
-wp. call(_:true). sim. wp. skip. progress.
-seq 1 1 : (aux_0{1} = i{2} /\ aux{1} = challenge_0{2}).
-sim.
-call (_: ={arg} ==> ={res}). proc. sim.
-call (_:true). wp.  while (={a,i}). wp.  skip. progress. wp. skip. progress.
-wp.  skip. progress.
-skip.  progress. wp.  auto.
-qed.
-
-require import BigNum_proofs.
-require import BigNum_spec.
-require import UniformSampling_Abstract.
-require import UniformSampling_Concrete.
-
-
-equiv rsample_cspec_equiv:
- M1.challenge_indexed ~ CSpecFp.rsample:
-   Constants.q = a{2}
-  ==> W64xN.valR res{1}.`2 = res{2}.`2 /\ res{1}.`1 = res{2}.`1.
-transitivity M2.challenge_indexed
- (={arg} ==> ={res})
- (Constants.q = a{2}
-  ==> W64xN.valR res{1}.`2 = res{2}.`2 /\ res{1}.`1 = res{2}.`1).
-progress. smt(). progress.
-conseq M1_M2_challenge. 
-proc*.
-inline M2.challenge_indexed.
-wp.
-call rsample_cspec.
-call {1} Constants.bn_set_q_correct.
-wp. skip. progress.
-qed.
-
-
-lemma challenge_cspec_pr  i x &m : 
-  Pr[ M1.challenge_indexed() @ &m : res = (i,x)  ]
-   = Pr[ CSpecFp.rsample(Constants.q) @ &m : res = (i, W64xN.valR x)  ].
-byequiv.
-conseq rsample_cspec_equiv. progress. progress. smt().
-smt(@W64xN). auto. auto.
-qed.
-
-
-lemma challenge_index_pos &m  : Pr[M1.challenge_indexed() @ &m : res.`1 <= 0 ] = 0%r.
-byphoare (_: true ==> _);auto. hoare.
-proc.  simplify.
-inline W64_SchnorrExtract_ct.M(W64_SchnorrExtract_ct.Syscall).bn_rsample.
-unroll 26. rcondt 26. wp. wp. 
-call (_:true). wp. auto. wp. 
-call (_:true). wp. auto. wp. skip. auto.
-wp.
-while (0 < i0). wp. call (_:true). auto. wp.  call (_:true). auto.  wp. 
-inline*. wp. rnd. wp. skip. progress.  smt().
-wp. call (_:true). auto.  wp.  
-call (_:true). auto. wp. 
-call (_:true). auto. wp. 
-call (_:true). auto. wp. 
-call (_:true). wp.  auto. wp.
-skip. progress. smt().
-qed.
-
-import W64xN.
-
-
-op g l : real 
- = if inv (-1) challenge_t l <= 0 then 0%r else 
-     mu D (predC (RSP Constants.q)) ^ (inv (-1) challenge_t l - 1)
-       * (1%r / W64xN.modulusR%r).
-
-        
-lemma leakfree1 &m x  l: (glob M1){m} = [] 
-  => Pr[ M1.challenge_indexed() @ &m : M1.leakages = l  /\ res.`2 = x  ] = if (Constants.q <= valR x) then 0%r else (g  l).
-      progress.
-   rewrite  (challenge_leakages_inv x l &m);auto.
-case (inv (-1) challenge_t l <= 0). 
-move => q. rewrite /g. rewrite q.  simplify. 
-  have : Pr[M1.challenge_indexed() @ &m :
-   inv (-1) challenge_t l = res.`1 /\ res.`2 = x] 
-    <= Pr[M1.challenge_indexed() @ &m : res.`1 <= 0 ]. simplify. rewrite Pr[mu_sub]. smt().
-   auto. smt(challenge_index_pos @Distr).
-move => q.
-have -> : 
- Pr[M1.challenge_indexed() @ &m :
-   inv (-1) challenge_t l = res.`1 /\ res.`2 = x]
-  = Pr[M1.challenge_indexed() @ &m :
-   res = (inv (-1) challenge_t l , x) ]. rewrite Pr[mu_eq]. smt(). auto.
-case (valR x < Constants.q) => case1.
-rewrite challenge_cspec_pr.
-rewrite rsample_pr.   smt().
-rewrite /RSP. auto.
-rewrite /z. 
-have ->: mu1 D (W64xN.valR x) = 1%r / W64xN.modulusR%r.
-rewrite duniform1E_uniq. smt(@List).
- have f1 : 0 <= W64xN.valR x < W64xN.modulusR. smt(@W64xN).  smt(@Distr @List). 
-rewrite /g.   smt().
-have : Pr[M1.challenge_indexed() @ &m :
-   res.`2 = x] = 0%r.
-  have -> : Pr[M1.challenge_indexed() @ &m :
-     res.`2 =  x] = Pr[ CSpecFp.rsample(Constants.q) @ &m : res.`2 =  W64xN.valR x ].
-  byequiv. conseq rsample_cspec_equiv. auto. progress. rewrite H0.  auto.  smt(@W64xN). auto. auto.
-  apply rsample_pr_out. auto.
-smt(@Distr).
-qed.
-
-
-op h : real = 1%r/Constants.q%r. 
-
-lemma leakfree2 &m x: 
- Pr[ M1.challenge_indexed() @ &m : res.`2 = x ] 
-  = if (Constants.q <= valR x) then 0%r else h .    
-proof. 
- have ->: Pr[ M1.challenge_indexed() @ &m : res.`2 = x ] =
-  Pr[ CSpecFp.rsample(Constants.q) @ &m : res.`2 =  W64xN.valR x ].
-  byequiv. conseq rsample_cspec_equiv. auto. 
-progress. rewrite - H. auto. smt(@W64xN). auto. auto.
-rewrite /h.
-case: (Constants.q <= valR x). move => alx.
-rewrite rsample_pr_out. smt(). auto.
-move => a_less_x.
-rewrite rsample_uni. auto. smt(@W64xN).
-smt(). auto.
-qed.
-
-op f l = h / g l.
-
-lemma rsample_leakfree_indexed l a &m: (glob M1){m} = [] 
- =>  let v = Pr[ M1.challenge_indexed() @ &m : res.`2 = a  ] in 
-     let w = Pr[ M1.challenge_indexed() @ &m : M1.leakages = l  /\ res.`2 = a  ] in 
-  0%r < w => v/w 
-  = f  l.
-move => l_empty v w f1.
-have : (valR a < Constants.q).
- case (Constants.q <= valR a) => h.
- have : w <= 0%r.
- rewrite /w.  
- rewrite (leakfree1 &m a l _). auto.
- rewrite h. auto.
- smt(). 
- smt().
-move => a_less_pin.
-rewrite /f.
-rewrite  (leakfree1 &m a l _). auto.
-rewrite  (leakfree2 &m a ). auto. 
-smt().
+apply challenge_leakages.
 qed.
 
 
@@ -284,19 +21,31 @@ lemma chalenge_leakfree l a &m: (glob M1){m} = []
  =>  let v = Pr[ M1.challenge() @ &m : res = a  ] in 
      let w = Pr[ M1.challenge() @ &m : M1.leakages = l  /\ res = a  ] in 
   0%r < w => v/w 
-  = f l.
-move => ge v w .
-have -> : Pr[ M1.challenge() @ &m : res = a  ] = Pr[ M1.challenge_indexed() @ &m : res.`2 = a  ].
-byequiv. proc. wp.
-wp. call (_:true). sim. 
-wp. call (_:true). sim. 
-wp.  skip. progress. auto. auto.
-
-have -> : Pr[ M1.challenge() @ &m : M1.leakages = l /\ res = a  ] = Pr[ M1.challenge_indexed() @ &m : M1.leakages = l /\ res.`2 = a  ].
-byequiv (_: ={M1.leakages} ==> _). proc. wp.
-wp. call (_: ={M1.leakages}). sim. 
-wp. call (_: ={M1.leakages}). sim. 
-wp.  skip. progress. auto. auto.
-apply (rsample_leakfree_indexed l a &m).
-auto. 
+  = 1%r.
+case (l = challenge_t).
+progress.
+ have ->: Pr[M(Syscall).challenge() @ &m : res = a] 
+  = Pr[M(Syscall).challenge() @ &m : res = a /\  M1.leakages = challenge_t ]
+  + Pr[M(Syscall).challenge() @ &m : res = a /\  M1.leakages <> challenge_t ].
+  rewrite Pr[mu_split (M1.leakages = challenge_t)]. auto.
+ have ->: Pr[M(Syscall).challenge() @ &m : res = a /\  M1.leakages <> challenge_t ] = 0%r.
+  have : Pr[M(Syscall).challenge() @ &m : res = a /\  M1.leakages <> challenge_t ]
+   <= Pr[M(Syscall).challenge() @ &m :  M1.leakages <> challenge_t ].
+   rewrite Pr[mu_sub]. smt(). auto.
+   have ->: Pr[M(Syscall).challenge() @ &m :  M1.leakages <> challenge_t ] = 0%r.
+   byphoare (_: M.leakages = [] ==> _). conseq (challenge_leakages_ph []). 
+   progress. smt(@List).  smt(@List).  auto. auto.
+   smt(@Distr). simplify. auto.
+ have ->: Pr[M(Syscall).challenge() @ &m : res = a /\ M.leakages = challenge_t] 
+   = Pr[M(Syscall).challenge() @ &m : M.leakages = challenge_t /\ res = a ]. rewrite Pr[mu_eq]. auto. auto.
+ smt(@Real).
+ progress.
+ have fact1 : 
+    Pr[M(Syscall).challenge() @ &m : M.leakages = l /\ res = a] = 
+    Pr[M(Syscall).challenge() @ &m : M.leakages = l /\ res = a /\ M.leakages <> challenge_t].
+ rewrite Pr[mu_eq]. smt(). auto.
+ have fact2 : Pr[M(Syscall).challenge() @ &m : M.leakages = l /\ res = a /\ M.leakages <> challenge_t] = 0%r.
+  byphoare (_: M.leakages = [] ==> _). proc*. call (challenge_leakages_ph []). skip. progress. 
+  smt(@List). auto. auto. 
+  smt().
 qed.
